proof/DeclarativeTyping.v
@@ -1,6 +1,20 @@
 Require Import CCP.Calculus.
 Require Import CCP.LiftSubst.
 Require Import CCP.Reduction.
+Require Import CCP.MyList.
+
+Definition env := list term.
+
+Implicit Type t T u U v V: term.
+Implicit Types i k m n p : nat.
+Implicit Types A B M N : term.
+Implicit Types e f g : env.
+Implicit Type G D : env.
+
+Definition item_lift t e n :=
+ex2 (fun u => t = lift (S n) u) (fun u => item term u (e:list term) n).
+
+Section Typing.
 
 (* Coercion judgment *)
 Inductive coerced : term -> term -> Prop :=
@@ -13,12 +27,11 @@ Inductive coerced : term -> term -> Prop :=
 
 Hint Resolve SubConv SubPi SubSigma SubLeft SubRight SubTrans : CCP.
 
-Definition ctx := list term.
 
-Inductive wfd : ctx -> Prop :=
+Inductive wfd : env -> Prop :=
   | WfEmpty : wfd nil
   | WfVar : forall G A s, typed G A (sort s) -> wfd (A :: G)
-with typed : ctx -> term -> term -> Prop :=
+with typed : env -> term -> term -> Prop :=
   | Var : forall G, wfd G -> 
     forall i, i < length G -> typed G (rel i) (lift i (nth i G sortS))
     
@@ -30,11 +43,12 @@ with typed : ctx -> term -> term -> Prop :=
     typed G (Pi A B) s -> typed (A :: G) x B ->
     typed G (lambda A x) (Pi A B)
 
-  | SortT : forall s t, SortR s t -> typed nil (sort s) (sort t)
+  | SortT : forall G, wfd G ->
+    forall s s', SortR s s' -> typed G (sort s) (sort s')
 
-  | App : forall G A B f x, 
-    typed G f (Pi A B) -> typed G x A ->
-    typed G (app f x) (subst x B)
+  | App : forall G A B u v, 
+    typed G u (Pi A B) -> typed G v A ->
+    typed G (app u v) (subst v B)
 
   | LetIn : forall G A B x y, typed G x A -> typed (A :: G) y B ->
     typed G (let_in x y) (subst x B)
@@ -55,11 +69,41 @@ with typed : ctx -> term -> term -> Prop :=
     typed G A sortS -> typed (A :: G) P sortP ->
     typed G (Subset A P) sortS
 
-  | Conv : forall G x A, 
-    typed G x A -> forall B, conv A B -> typed G x B
-
   | Subsum : forall G x A, 
     typed G x A -> forall B, coerced A B -> typed G x B.
+
+Notation "G |- t : T" := (typed G t T) (at level 50).
+Notation "T >> U" := (coerced T U) (at level 50).
+Notation "|-  G" := (wfd G) (at level 50).
+
+
+Lemma type_prop_set :
+   forall s, is_propset s -> forall e, wfd e -> typed e (sort s) (sortT 0).
+unfold sortT ; simple destruct 1; intros; rewrite H0.
+apply SortT; trivial.
+constructor.
+apply SortT; trivial.
+constructor.
+Qed.
+
+Lemma typ_free_db : forall e t T, typed e t T -> free_db (length e) t.
+simple induction 1; intros; auto with CCP core arith datatypes.
+inversion_clear H1.
+apply db_rel.
+elim H3; simpl in |- *; intros; auto with coc core arith datatypes.
+Qed.
+
+
+  Lemma typ_wf : forall e t T, typ e t T -> wf e.
+simple induction 1; auto with coc core arith datatypes.
+Qed.
+
+
+
+
+
+
+
 
 
 Fixpoint lift_ctx_rec (n k : nat) (G : ctx) { struct G } : ctx :=
@@ -70,29 +114,40 @@ Fixpoint lift_ctx_rec (n k : nat) (G : ctx) { struct G } : ctx :=
 
 Definition lift_ctx (n : nat) (G : ctx) := lift_ctx_rec n (length G) G.
 
+Fixpoint subst_ctx_rec (t : term) (k : nat) (G : ctx) { struct k } : ctx := 
+  match k with
+  | 0 => G
+  | S k' =>
+    match G with
+    | nil => nil
+    | cons u G' => subst_rec t u k' :: (subst_ctx_rec t k' G')
+    end
+  end.
+
+Definition subst_ctx (t : term) (G : ctx) := subst_ctx_rec t (length G) G.
+
 Hint Unfold lift_ctx lift_ctx_rec : CCP.
 
 Hint Resolve WfEmpty WfVar : CCP.
-Hint Resolve Var Prod Abs SortT App LetIn Sum Pair LetTuple SubsetI Conv Subsum : CCP.
+Hint Resolve Var Prod Abs SortT App LetIn Sum Pair LetTuple SubsetI Subsum : CCP.
 
 Scheme typed_mut := Induction for typed Sort Prop
 with wfd_mut := Induction for wfd Sort Prop.
 
 Scheme typed_depind := Induction for typed Sort Prop.
-Check typed_mut.
 
 Lemma typed_wf : forall G t T, typed G t T -> wfd G.
 Proof.
   induction 1 ; autoc.
 Qed.
 
-Lemma coercion_sym : forall T U, coerced T U -> coerced U T.
+Lemma coercion_sym : forall T U, T >> U -> U >> T.
 Proof.
   induction 1 ; autoc.
   apply SubTrans with B ; autoc.
 Qed.
 
-Lemma coercion_conversion : forall U T V, coerced T U -> conv U V -> coerced T V.
+Lemma coercion_conversion : forall U T V, T >> U -> conv U V -> T >> V.
 Proof.
   intros.
   apply SubTrans with U ; autoc.
@@ -128,11 +183,163 @@ Proof.
 Qed. 
 
 Require Import CCP.ListProps.
+Require Import Arith.
 
-Lemma weakening : forall G t T U,  wfd (U :: G) ->  
+Lemma wf_sort :
+   forall n e f,
+   trunc _ (S n) e f ->
+   wf e -> forall t, item _ t e n -> exists s : sort, typ f t (Srt s).
+simple induction n.
+do 3 intro.
+inversion_clear H.
+inversion_clear H0.
+intros.
+inversion_clear H0.
+inversion_clear H.
+exists s; auto with coc core arith datatypes.
+
+do 5 intro.
+inversion_clear H0.
+intros.
+inversion_clear H2.
+inversion_clear H0.
+elim H with e0 f t; intros; auto with coc core arith datatypes.
+exists x0; auto with coc core arith datatypes.
+
+apply typ_wf with x (Srt s); auto with coc core arith datatypes.
+Qed.
+
+
+
+
+Lemma substitution : forall G A a, typed G a A ->
+  forall G' t T, typed G' t T ->
+  forall D, G' = D ++ A :: G -> let n := length D in  
+  typed (subst_ctx_rec a n (D ++ G)) 
+    (subst_rec a t n) (subst_rec a T n).
+Proof.
+  intros G A a Ha.
+  intros G' t T Ht.
+  induction Ht using typed_mut with 
+  (P := fun G' : ctx => fun t T : term => fun H : typed G' t T =>
+  forall D, G' = D ++ A :: G -> let n := length D in  
+  typed (subst_ctx_rec a n (D ++ G))
+    (subst_rec (lift (S n) a) t n) (subst_rec (lift (S n) a) T n)) 
+  (P0 := fun G' : ctx => fun H : wfd G' =>
+  forall D, G' = D ++ A :: G -> let n := length D in  
+  wfd (subst_ctx_rec a n (D ++ G))).
+  intros.
+  
+  induction D.
+  simpl in n.
+  unfold n.
+  case i.
+  simpl.
+  rewrite lift_0.
+  rewrite lift_0.
+  rewrite H.
+  simpl.
+  
+  unfold lift.  
+  
+rewrite simpl_subst_rec.
+
+  simpl.
+  elim (lt_eq_lt_dec i 0) ; intros.
+  induction a0.
+  elim (lt_n_O _ a0).
+  rewrite b.
+  rewrite lift_0.
+  rewrite lift_0.
+  rewrite H.
+  simpl.
+  unfold lift ; rewrite simpl_subst_rec ; auto with arith.
+  rewrite lift_rec_0.
+  apply Ha.
+  unfold lift ; rewrite simpl_subst_rec ; auto with arith.
+  rewrite simpl_lift_rec ; simpl ; auto with arith.
+  rewrite H.
+  simpl.
+  elim i.
+
+  simpl.
+
+  simpl in H.
+  rewrite H in w.
+  inversion w.
+
+  simpl in n.
+
+
+  unfold n ; simpl.
+  
+  Focus 2.
+  
+
+  rewrite subst_rec_0.
+
+
+  induction Ht using typed_mut with 
+  (P := fun G : ctx => fun t T : term => fun H : typed G t T =>
+  typed (subst_ctx_rec a n G) 
+    (subst_rec a t n) (subst_rec a T n)).
+
+  (P0 := 
+  (fun G : ctx => fun x : wfd G =>
+  forall U,
+  wfd (U :: G) ->
+  forall m, forall G' : ctx, m = length G' ->
+  wfd (G' ++ G) ->
+  wfd ((lift_ctx_rec 1 m G') ++ (U :: G)))).
+
+) (Q :=   /\ (wfd (D ++ A :: G) -> wfd (subst_ctx a D ++ G)))
+
+  induction D.
+
+  simpl.
+  elim (lt_eq_lt_dec i 0) ; intros.
+  induction a0.
+  elim (lt_n_O i a0).
+  rewrite b.
+  rewrite lift_0.
+  rewrite lift_0.
+  
+
+  unfold lift ; simpl.
+
+  induction i.
+
+
+Lemma subject_reduction : forall G t t' T, (typed G t T) -> red t t' -> 
+  (typed G t' T).
+Proof.
+  intros.
+  induction H0.
+  assumption.
+  induction H1.
+  inversion IHred.
+  inversion H4.
+  
+
+Lemma unicity_sorting : forall G T s s', 
+  (typed G T (sort s) /\ typed G T (sort s')) -> s = s'.
+Proof.
+  induction T.
+  intros.
+  induction H.
+  inversion H ; inversion H0.
+  rewrite H2 in H7.
+  injection H7 ; auto.
+  
+  
+
+Lemma weakening : forall G t T U,
+  (|- (U :: G)) ->  
   forall m G',
   m = length G' ->
-  typed (G' ++ G) t T -> typed ((lift_ctx_rec 1 m G') ++ (U :: G)) (lift_rec 1 t m) (lift_rec 1 T m).
+  typed (G' ++ G) (lift m t) (lift m T) -> 
+  typed ((lift_ctx_rec 1 m G') ++ (U :: G)) 
+         (lift (S m) t) (lift (S m) T).
 Proof.
   intros G t T.
   apply typed_mut with 
@@ -141,8 +348,9 @@ Proof.
   forall U, 
   wfd (U :: G) ->
   forall m, forall G' : ctx,  m = length G' ->
-  typed (G' ++ G) t T ->
-  typed ((lift_ctx_rec 1 m G') ++ (U :: G)) (lift_rec 1 t m) (lift_rec 1 T m))
+  typed (G' ++ G) (lift m t) (lift m T) ->
+  typed ((lift_ctx_rec 1 m G') ++ (U :: G)) 
+    (lift (S m) t) (lift (S m) T))
   (P0 := 
   (fun G : ctx => fun x : wfd G =>
   forall U,
@@ -152,18 +360,60 @@ Proof.
   wfd ((lift_ctx_rec 1 m G') ++ (U :: G)))).
   
   intros.
+  set (G'' := lift_ctx_rec 1 m G'). 
   simpl.
-  elim (le_gt_dec m i) ; auto ; intros.
-  unfold lift ; rewrite simpl_lift_rec ; auto with arith.
-  simpl.
-  cut(nth i G0 sortS = nth (m + S i) (lift_ctx_rec 1 m G' ++ U :: G0) sortS).
+  cut(nth i G0 sortS = nth (S m + i) (G'' ++ U :: G0) sortS).
   intros.
   rewrite H3.
-  pose (v := Var) ; unfold lift in v.
-  induction m.
   simpl.
-  apply v ; rewrite (length_0_nil _ G' (sym_eq H1)) ; simpl ; auto with arith.
+  pose (v := Var) ; unfold lift in v.
+  unfold lift ; rewrite simpl_lift_rec ; auto with arith.
+  elim (le_gt_dec m i) ; intros Hmi ; simpl.
+  apply v.
+  unfold G'' ; apply H ; auto.
+  apply (typed_wf _ _ _ H2).
+  rewrite length_app.
+  unfold G'' ; rewrite lift_ctx_rec_length.
+  rewrite <- H1.
+  simpl.
+  omega.
+  apply v.
+  unfold G'' ; apply H ; auto.
+  apply (typed_wf _ _ _ H2).
+  rewrite length_app.
+  unfold G'' ; rewrite lift_ctx_rec_length.
+  rewrite <- H1.
+  simpl.
+  omega.
+  cut(S m = length (G'' ++ U :: nil)).
+  intros. 
   rewrite H3.
+  assert(G'' ++ U :: G0 = (G'' ++ U :: nil) ++ G0).
+  rewrite <- ass_app ; auto.
+  rewrite H4.
+  apply nth_i_app.
+  rewrite length_app.
+  simpl.
+  unfold G'' ; rewrite lift_ctx_rec_length ; rewrite H1; rewrite plus_comm ; auto with arith.
+
+  (* Pi *)
+  intros.
+  unfold lift ; simpl ; unfold lift in H, H0 ; simpl in H, H0.
+  eapply Prod.
+  apply H ; auto.
+  inversion H3.
+
+  apply 
+  
+  unfold lift ; simpl.
+  rewrite simpl_lift_rec ; auto with arith.
+  
+
+  induction G'.
+  simpl.
+  simpl in H1 ; rewrite H1.
+  auto.
+
 
 
 
